compiler/src/FlatImp.v
@@ -593,6 +593,13 @@ Section FlatImp2.
   Context {pp : unique! Semantics.parameters}.
   Context {ok : Semantics.parameters_ok pp}.
 
+  Definition SimState: Type := env * stmt * bool * trace * mem * locals.
+  Definition SimExec: SimState -> (SimState -> Prop) -> Prop :=
+    fun '(e, c, done, t, m, l) post =>
+      done = false /\
+      forall mc, exec e c t m l mc (fun t' m' l' mc' =>
+                                      post (e, c, true, t', m', l')).
+
   Lemma increase_fuel_still_Success: forall fuel1 fuel2 e initialSt initialM s final,
     (fuel1 <= fuel2)%nat ->
     eval_stmt e fuel1 initialSt initialM s = Some final ->
